verifier/src/main/java/com/aws/jverify/verifier/compiler/dafnygenerator/base/TypeDeclarationCompiler.java
@@ -433,8 +433,7 @@ public class TypeDeclarationCompiler {
             var parameterSymbol = parameterSymbols.get(index);
             IOrigin parameterOrigin = compiler.toOrigin(parameter);
             Name formalName = new Name(parameterOrigin, compiler.nameCompiler.getCompiledName(parameter.sym, parameter));
-            // TODO use parameter.sym.type ?
-            var syntacticType = compiler.translateMethodSignatureType(parameterSymbol.type, parameterOrigin, shouldVerify);
+            var syntacticType = compiler.translateMethodSignatureType(parameter.sym.type, parameterOrigin, shouldVerify);
             return new Formal(parameterOrigin, formalName, syntacticType, false, true,
                     null, null, false, false, false, null);
         }).toList();
